src/rocq/Utils/RaiseCtree.v
@@ -1,0 +1,238 @@
+From Stdlib Require Import
+     String
+     Morphisms.
+
+From ExtLib Require Import
+     Structures.Monads.
+
+Unset Universe Checking.
+From Vellvm Require Import 
+  Semantics.LLVMEvents
+  Utils.Tactics
+  Utils.Raise
+  Utils.Error
+  Utils.CTreeUtils.
+
+Unset Universe Checking.
+From CTree Require Import
+  CTree CTreeDefinitions Eq.
+
+Require Import Stdlib.Program.Equality.
+
+Require Import Paco.paco.
+
+Import MonadNotation.
+Open Scope monad.
+
+
+(* TODO: Move this *)
+Definition raise {E B} {A} `{FailureE -< E} (msg : String.string) : ctree E B A :=
+  (v <- trigger (Throw (print_msg msg));; match v: void with end)%monad.
+
+(* TODO: Move this *)
+#[global] Instance RAISE_ERR_CTREE_FAILUREE {E B : Type -> Type} `{FailureE -< E} : RAISE_ERROR (ctree E B) :=
+  { raise_error := fun A e => raise e
+  }.
+
+(* TODO: Move this *)
+Definition raiseUB {E B} {A} `{UBE -< E} (msg : String.string) : ctree E B A :=
+  v <- trigger (ThrowUB (print_msg msg));; match v: void with end.
+
+(* TODO: Move this *)
+#[global] Instance RAISE_UB_CTREE_FAILUREE {E B : Type -> Type} `{UBE -< E} : RAISE_UB (ctree E B) :=
+  { raise_ub := fun A e => raiseUB e
+  }.
+
+(* TODO: Move this *)
+Definition raiseOOM {E B} {A} `{OOME -< E} (msg : String.string) : ctree E B A :=
+  v <- trigger (ThrowOOM (print_msg msg));; match v: void with end.
+
+(* TODO: Move this *)
+#[global] Instance RAISE_OOM_CTREE_FAILUREE {E B : Type -> Type} `{OOME -< E} : RAISE_OOM (ctree E B) :=
+  { raise_oom := fun A e => raiseOOM e
+  }.
+
+(* #[global] Instance Reflexive {F X} : Reflexive (@update_val_rel F F X X eq eq). *)
+(* red. *)
+(* intros x. *)
+(* Set Printing Implicit. *)
+(* apply update_val_rel_eq; eauto. *)
+(* - destruct x; cbn. *)
+(*   + apply wf_val_nonval. *)
+(*     apply is_val_τ. *)
+(*   + apply wf_val_nonval. *)
+(*     apply is_val_obs. *)
+(*   + eapply wf_val_val. *)
+(*     apply is_val_obs. *)
+(* -destruct x; try constructor; eauto. *)
+(* constructor. *)
+(* apply update_val_rel_eq; eauto. *)
+(* Qed. *)
+
+Section Failure.
+  Variable E : Type -> Type.
+  Variable B : Type -> Type.
+  Context {FAIL : FailureE -< E}.
+
+  Lemma raise_bind_ctree :
+    forall X Y (f : X -> ctree E B Y) x,
+      bind (raise x) f ~ (raise x : ctree E B Y).
+  Proof using.
+    intros X Y f x.
+    cbn.
+    rewrite bind_bind.
+    eapply sbisim_clo_bind_eq; [|intros []].
+    reflexivity.
+  Qed.
+
+  Lemma raise_map_ctree :
+    forall X Y (f : X -> Y) x,
+      CTree.map f (@raise _ _ _ FAIL x : ctree E B X) ~ (raise x : ctree E B Y).
+  Proof using.
+    intros X Y f x.
+    unfold raise.
+    setoid_rewrite map_bind.
+    eapply sbisim_clo_bind_eq.
+    reflexivity.
+    intros [].
+  Qed.
+
+  Lemma raise_map_ctree_inv :
+    forall X Y (f : X -> Y) (t : ctree E B X) x,
+      CTree.map f t ~ (@raise _ _ _ FAIL x : ctree E B Y) ->
+      t ~ (raise x : ctree E B X).
+  Proof using.
+    intros X Y f t x H.
+    unfold CTree.map in *.
+  Admitted.
+
+  Lemma raise_ret_inv_ctree :
+      forall A x (y : A),
+        ~ (@raise _ _ _ FAIL x : ctree E B A) ~ (ret y : ctree E B A).
+  Proof using.
+    intros A x y.
+    intros CONTRA.
+    symmetry in CONTRA.
+    unfold raise in CONTRA.
+    setoid_rewrite bind_trigger in CONTRA.
+    apply sbisim_ret_vis_inv in CONTRA.
+    auto.
+  Qed.
+
+  #[global] Instance RaiseBindM_Fail : RaiseBindM (ctree E B) string (fun T => raise) :=
+    { rbm_raise_bind := raise_bind_ctree;
+      rbm_raise_ret_inv := raise_ret_inv_ctree;
+    }.
+End Failure.
+
+Section OOM.
+  Variable E : Type -> Type.
+  Variable B : Type -> Type.
+  Context {OOM : OOME -< E}.
+
+  Lemma raiseOOM_bind_ctree :
+    forall X Y (f : X -> ctree E B Y) x,
+      bind (raiseOOM x) f ~ (raiseOOM x : ctree E B Y).
+  Proof using.
+    intros X Y f x.
+    cbn.
+    rewrite bind_bind.
+    eapply sbisim_clo_bind_eq; [|intros []].
+    reflexivity.
+  Qed.
+
+  Lemma raiseOOM_map_ctree :
+    forall X Y (f : X -> Y) x,
+      CTree.map f (@raiseOOM _ _ _ OOM x : ctree E B X) ~ (raiseOOM x : ctree E B Y).
+  Proof using.
+    intros X Y f x.
+    unfold raise.
+    setoid_rewrite map_bind.
+    eapply sbisim_clo_bind_eq.
+    reflexivity.
+    intros [].
+  Qed.
+
+  Lemma raiseOOM_map_ctree_inv :
+    forall X Y (f : X -> Y) (t : ctree E B X) x,
+      CTree.map f t ~ (@raiseOOM _ _ _ OOM x : ctree E B Y) ->
+      t ~ (raiseOOM x : ctree E B X).
+  Proof using.
+    intros X Y f t x H.
+    unfold CTree.map in *.
+  Admitted.
+
+  Lemma raiseOOM_ret_inv_ctree :
+      forall A x (y : A),
+        ~ (@raiseOOM _ _ _ OOM x : ctree E B A) ~ (ret y : ctree E B A).
+  Proof using.
+    intros A x y.
+    intros CONTRA.
+    symmetry in CONTRA.
+    unfold raise in CONTRA.
+    setoid_rewrite bind_trigger in CONTRA.
+    apply sbisim_ret_vis_inv in CONTRA.
+    auto.
+  Qed.
+
+  #[global] Instance RaiseBindM_OOM : RaiseBindM (ctree E B) string (fun T => raiseOOM) :=
+    { rbm_raise_bind := raiseOOM_bind_ctree;
+      rbm_raise_ret_inv := raiseOOM_ret_inv_ctree;
+    }.
+End OOM.
+
+Section UB.
+  Variable E : Type -> Type.
+  Variable B : Type -> Type.
+  Context {UB : UBE -< E}.
+
+  Lemma raiseUB_bind_ctree :
+    forall X Y (f : X -> ctree E B Y) x,
+      bind (raiseUB x) f ~ (raiseUB x : ctree E B Y).
+  Proof using.
+    intros X Y f x.
+    cbn.
+    rewrite bind_bind.
+    eapply sbisim_clo_bind_eq; [|intros []].
+    reflexivity.
+  Qed.
+
+  Lemma raiseUB_map_ctree :
+    forall X Y (f : X -> Y) x,
+      CTree.map f (@raiseUB _ _ _ UB x : ctree E B X) ~ (raiseUB x : ctree E B Y).
+  Proof using.
+    intros X Y f x.
+    unfold raise.
+    setoid_rewrite map_bind.
+    eapply sbisim_clo_bind_eq.
+    reflexivity.
+    intros [].
+  Qed.
+
+  Lemma raiseUB_map_ctree_inv :
+    forall X Y (f : X -> Y) (t : ctree E B X) x,
+      CTree.map f t ~ (@raiseUB _ _ _ UB x : ctree E B Y) ->
+      t ~ (raiseUB x : ctree E B X).
+  Proof using.
+    intros X Y f t x H.
+    unfold CTree.map in *.
+  Admitted.
+
+  Lemma raiseUB_ret_inv_ctree :
+      forall A x (y : A),
+        ~ (@raiseUB _ _ _ UB x : ctree E B A) ~ (ret y : ctree E B A).
+  Proof using.
+    intros A x y.
+    intros CONTRA.
+    symmetry in CONTRA.
+    unfold raise in CONTRA.
+    setoid_rewrite bind_trigger in CONTRA.
+    apply sbisim_ret_vis_inv in CONTRA.
+    auto.
+  Qed.
+
+  #[global] Instance RaiseBindM_UB : RaiseBindM (ctree E B) string (fun T => raiseUB) :=
+    { rbm_raise_bind := raiseUB_bind_ctree;
+      rbm_raise_ret_inv := raiseUB_ret_inv_ctree;
+    }.
+End UB.
